helping/HelpingOn.v
@@ -1,59 +1,57 @@
 Require Import CRIS SchHeader.
-Require Import HelpingHeader.
+From CRIS.helping Require Import Header.
 
-Set Implicit Arguments.
+Module HelpingOn. Section HelpingOn.
 
-Module HelpingOn.
-Section HelpingOn.
-  Context `{Σ: GRA}.
+  Context `{Σ : GRA}.
 
-  Variable mn: string.
-  Variable jobID : Type.
-  Variable jobcode : jobID -> itree Helping.pureE unit.
+  Context (mn : string).
+  Context {jobID : Type} (jobcode : jobID → itree Helping.pureE unit).
 
-  Definition joblist : Type := list (nat * jobID).
-  
+  Definition jobmap : Type := gmap nat jobID.
+
   Definition scopes := [mn].
   Definition v_reqs := mn ↯ "reqs".
 
-  Definition try_run tid : itree hmodE Any.t :=
-    'reqs: joblist <- cgetU v_reqs;;
-    match alist_find tid reqs with
+  Definition try_run (tid : nat) : itree crisE Any.t :=
+    'reqs : jobmap <- cgetU v_reqs;;
+    match reqs !! tid with
     | None => Ret ()↑
     | Some jid =>
-        cput v_reqs (alist_remove tid reqs : joblist);;;
+        cput v_reqs (delete tid reqs);;;
         Helping.trans (jobcode jid);;;
         Ret ()↑
     end.
 
-  Definition run: Any.t -> itree hmodE Any.t :=
-    fun arg =>
-      'jid: jobID <- arg↓?;;
-      'tid: nat <- ccallU SchHdr.get_tid ();;
-      'reqs: joblist <- cgetU v_reqs;;
-      cput v_reqs (alist_add tid jid reqs : joblist);;;
+  Definition run: Any.t → itree crisE Any.t :=
+    λ arg,
+      'jid : jobID <- arg↓?;;
+      'tid : nat <- ccallU SchHdr.get_tid ();;
+      'reqs : jobmap <- cgetU v_reqs;;
+      cput v_reqs (<[tid := jid]> reqs);;;
       𝒴;;;
       try_run tid.
 
-  Definition help: Any.t -> itree hmodE Any.t :=
-    fun _ =>
+  Definition help: Any.t → itree crisE Any.t :=
+    λ _,
       𝒴;;;
       tid <- trigger (Choose nat);;
-      try_run tid.
-      
-  Definition fnsems :=
-    [(Helping.run mn,  (wmask_all, scopes, mk_specbody fspec_trivial run));
-     (Helping.help mn, (wmask_all, scopes, mk_specbody fspec_trivial help))].
+      try_run tid;;;
+      𝒴;;;
+      Ret ()↑.
+
+  Definition fnsems : alist (option string) (fnsem_type (option fspec * fbody)) :=
+    [(Some (Helping.run mn),  (false, wmask_all, scopes, (None, run)));
+     (Some (Helping.help mn), (false, wmask_all, scopes, (None, help)))].
 
   Program Definition Mod: SMod.t := {|
     SMod.scopes := scopes;
     SMod.fnsems := fnsems;
-    SMod.initial_st := [(v_reqs, ([]: joblist)↑)];
+    SMod.initial_st := [(v_reqs, (∅ : jobmap)↑)];
   |}.
   Solve All Obligations with prove_scope.
   Next Obligation. prove_nodup. Qed.
 
-  Definition t sp := Seal.sealing CRIS (SMod.to_hmod sp Mod).  
-  
-End HelpingOn.
-End HelpingOn.
+  Definition t sp : Mod.t := Seal.sealing CRIS (SMod.to_mod sp Mod).
+
+End HelpingOn. End HelpingOn.
