helping/Header.v
@@ -1,0 +1,18 @@
+Require Import CRIS.
+
+Module Helping. Section Helping.
+
+  Context `{Σ: GRA}.
+  Context (mn : string).
+
+  Definition run  := mn +:+ ".run".
+  Definition help  := mn +:+ ".help".
+
+  Definition pureE := agE +' coreE.
+
+  Definition trans {R} (itr: itree pureE R) : itree crisE R :=
+    translate (case_ (bif:=sum1) subevent subevent) itr.
+
+  Definition exports := [run; help].
+
+End Helping. End Helping.
