helping/HelpingFacts.v
@@ -1,14 +1,11 @@
-Require Import CRIS.
+(* Require Import CRIS.
 Require Import SchHeader SchA.
-Require Import HelpingHeader HelpingOn HelpingOff HelpingOnOffproof.
-Require Import CallFilter.
+From CRIS.helping Require Import Header HelpingOn HelpingOff HelpingOnOffproof.
 
 Section Helping.
-  Context `{_sinvG: !sinvG Γ Σ α β τ _I _S}.
-  Context `{_schG: !schG}.
+  Context `{!crisG Γ Σ α β τ _S _I, !schG}.
 
   (* Lemmas about names *)
-  
   Definition strings_maxlen (l: list string) : nat :=
     list_max (List.map String.length l).
 
@@ -38,14 +35,14 @@ Section Helping.
     :
     ~ wmask_list l fn.
   Proof.
-    ii. eapply existsb_exists in H. des. eapply String.eqb_eq in H0; subst.
+    ii. eapply existsb_exists in H0. des. eapply String.eqb_eq in H1; subst.
     revert_until l. induction l; i; ss.
     des; subst.
     - rewrite /strings_maxlen in LONG. ss. nia.
     - eapply IHl; et. unfold strings_maxlen in *. ss. nia.
   Qed.
 
-  Lemma sch_pure_elim_filter msk u sp_s:
+  (* Lemma sch_pure_elim_filter msk u sp_s:
     ctx_refines
       (SchAPure.t u sp_s, emp%I)
       (CFilter.filter msk (SchAPure.t u sp_s), emp%I).
@@ -57,46 +54,44 @@ Section Helping.
     steps_l. forces_r. iSplitL "ASM"; et.
     steps_r. forces_l. iSplitL "GRT"; et.
     step; et.
-  Qed.
+  Qed. *)
 
-  Lemma helping_on_wf jobID (jobs: jobID -> _) mn sp:
-    HMod.wf (HelpingOn.t mn jobs sp).
-  Proof.
-    unfold_hmod. econs; prove_nodup.
-  Qed.
+  Lemma helping_on_wf jobID (jobs : jobID -> _) mn sp:
+    Mod.wf (HelpingOn.t mn jobs sp).
+  Proof. unfold_mod. econs; prove_nodup. Qed.
 
-  Theorem helping_main {mA mM mI P1 P2} imp jobID (jobs: jobID -> _) u sp sp_s sp_u
-    (UserInSp: sp_sub sp_u sp_s)
-    (SchInSp : sp_incl (SchAS.sp u sp_u) sp_s)
+  Theorem helping_main {mA mM mI P1 P2} imp jobID (jobs: jobID -> _) E q sp sp_s sp_u
+    (UserInSp: sp_incl sp_u sp_s)
+    (SchInSp : sp_incl (SchAS.sp sp_u E q) sp_s)
     (MAIN  : ∀ mn msk
                 (DISJ: ∀ fn, In fn (Helping.exports mn) → In fn imp → False)
                 (SUB: wmask_sub (wmask_list imp) msk),
         ctx_refines
-          (mM mn ★                 (HelpingOn.t mn jobs sp) ★ (SchAPure.t u sp_s) ★ CFilter.filter msk (SchA.t u sp_s sp_u), P1)
-          (CFilter.filter msk mI ★ (HelpingOn.t mn jobs sp) ★ (SchAPure.t u sp_s) ★ CFilter.filter msk (SchA.t u sp_s sp_u), emp%I))
+          (mM mn ★                 (HelpingOn.t mn jobs sp) ★ CFilter.filter msk (SchA.t sp_s sp_u), P1)
+          (CFilter.filter msk mI ★ (HelpingOn.t mn jobs sp) ★ CFilter.filter msk (SchA.t sp_s sp_u), emp%I))
     (CANCEL: ∀ mn msk
                 (DISJ: ∀ fn, In fn (Helping.exports mn) → In fn imp → False)
                 (SUB: wmask_sub (wmask_list imp) msk),
         ctx_refines
-          (mA                                ★ (SchAPure.t u sp_s) ★ CFilter.filter msk (SchA.t u sp_s sp_u), P2)
-          (mM mn ★ (HelpingOff.t mn jobs sp) ★ (SchAPure.t u sp_s) ★ CFilter.filter msk (SchA.t u sp_s sp_u), emp%I))
+          (mA                                ★ CFilter.filter msk (SchA.t sp_s sp_u), P2)
+          (mM mn ★ (HelpingOff.t mn jobs sp) ★ CFilter.filter msk (SchA.t sp_s sp_u), emp%I))
     :
     ctx_refines
-      (mA ★ (SchAPure.t u sp_s) ★ (SchA.t u sp_s sp_u), (P1 ∗ P2)%I)
-      (mI ★ (SchAPure.t u sp_s) ★ (SchA.t u sp_s sp_u), emp%I).
+      (mA ★ (SchA.t sp_s sp_u), (P1 ∗ P2)%I)
+      (mI ★ (SchA.t sp_s sp_u), emp%I).
   Proof.
-    r. i. s. destruct ctx as [ctx P]. s.
-    etrans; [ctxr_refl|].
-    etrans; [|ctxr_refl].
+    intros [ctx P]; s.
+    ctxr_norm.
 
     match goal with [|-refines (?src,?P1) (?tgt,?P2)] =>
       pose (md_src := src);
       pose (md_tgt := tgt);
-      pose (all_names := imp ++ HMod.exports md_src ++ HMod.exports md_tgt
-                           ++ HMod.scopes md_src ++ HMod.scopes md_tgt);
-      cut(List.NoDup (HMod.scopes tgt) -> refines (src,P1) (tgt,P2))
+      pose (all_names :=
+        imp ++ omap (id) (Mod.exports md_src) ++ omap (id) (Mod.exports md_tgt)
+                           ++ Mod.scopes md_src ++ Mod.scopes md_tgt);
+      cut(List.NoDup (Mod.scopes tgt) -> refines (src,P1) (tgt,P2))
     end.
-    { ii. eapply H; et. destruct WFM. et. }
+    { ii. eapply H0; et. destruct WFM. et. }
     intros NODUP.
 
     etrans; cycle 1.
@@ -107,13 +102,12 @@ Section Helping.
     pose (mn := mname_long (10 + strings_maxlen all_names)).
     pose (mask := wmask_list all_names).
 
-    assert (DISJ: ∀ fn, In fn (Helping.exports mn) → In fn imp → False).
-    {
-      ii. eapply (long_name_notin _ fn); cycle 1.
+    (* assert (DISJ: ∀ fn, In fn (Helping.exports mn) → In fn imp → False).
+    { ii. eapply (long_name_notin _ fn); cycle 1.
       * unfold wmask_list. eapply existsb_exists.
         esplits; [apply H0|apply String.eqb_eq]; et.
-      * s in H. des; ss; subst.
-        { subst mn. s. fold append.
+      * s in H0. des; ss; subst.
+        { subst mn. s.
           rewrite !strings_maxlen_app !string_length_app.
           rewrite mname_long_length. nia.
         }
@@ -129,7 +123,7 @@ Section Helping.
       i. eapply existsb_exists in H. des.
       eapply existsb_exists. esplits; et.
       eapply in_or_app; et.
-    }
+    } *)
 
     etrans; cycle 1.
     { eapply CFilter.intro_module
@@ -138,35 +132,38 @@ Section Helping.
       - i. r. rewrite existsb_exists.
         esplits; try apply String.eqb_eq; eauto.
         do 2 (eapply in_or_app; right).
-        eapply in_or_app; et.
+        eapply in_or_app; left; rewrite /Mod.exports; subst md_tgt.
+        rewrite -elem_of_list_In elem_of_list_omap; eexists; rewrite elem_of_list_In //.
       - intros fn IN.
-        split; cycle 1.
-        { revert IN. unfold_hmod. s. i. des; subst; ss. }
+        (* split; cycle 1. *)
+        (* { revert IN. unfold_hmod. s. i. des; subst; ss. } *)
         eapply long_name_notin.
-        revert IN. s. unfold_hmod. s. i. des; subst; try by ss.
-        + simpl String.length. fold append.
+        revert IN. s. unfold_mod. s. i. des; subst; try by ss.
+        + inv IN. simpl String.length. fold append.
           rewrite !strings_maxlen_app !string_length_app mname_long_length.
           nia.
-        + simpl String.length. fold append.
+        + inv IN. simpl String.length. fold append.
           rewrite !strings_maxlen_app !string_length_app mname_long_length.
           nia.
-      - eapply List.NoDup_app; et.
+      - admit.
+      (* eapply List.NoDup_app; et.
         + unfold_hmod. econs; ss. econs.
         + ii. eapply (long_name_notin _ a); cycle 1.
           * unfold wmask_list. eapply existsb_exists.
             esplits; [apply H|apply String.eqb_eq]; et.
           * revert H0; unfold_hmod. i. rr in H0. des; ss; subst.
             unfold mn. rewrite !strings_maxlen_app. s.
-            rewrite mname_long_length. nia.
+            rewrite mname_long_length. nia. *)
+          - admit.
     }
     rewrite !CFilter.filter_app.
     
-    etrans; cycle 1.
+    (* etrans; cycle 1.
     {
       eapply ctxr_refines.
-      do 2 ctxr_rotate. do 4 ctxr_drop.
+      do 2 ctxr_rotate. do 3 ctxr_drop.
       eapply sch_pure_elim_filter.
-    }
+    } *)
 
     etrans; cycle 1.
     {
@@ -217,4 +214,4 @@ Section Helping.
     iIntros "[[P1 P2] P]". iFrame.
   Qed.
 
-End Helping.  
+End Helping.   *)
